

1. **(Problem-solving):** For the grammar:

### Step-by-Step Derivation

1. Start with **S**.
2. Expand **S**  $\rightarrow$  **AB**.
3. Expand **A** to get the three 'a's':
  - $A \rightarrow aA$
  - $A \rightarrow aA \rightarrow aaA$
  - $A \rightarrow aA \rightarrow aaA \rightarrow aaaA$
  - Finally,  $A \rightarrow \varepsilon$  (the last A becomes empty).
4. Expand **B** to get the single 'b':
  - $B \rightarrow bB$
  - $B \rightarrow \varepsilon$  (the last B becomes empty).

Step	stack	input	Action
1.	\$	aaab\$	start
2.	\$a	aab\$	shift
3.	\$aa	ab\$	shift
4.	\$aa	b\$	shift
5.	\$aaab	\$	shift
6.	\$aaab	\$	Reduce $A \rightarrow \varepsilon$
7.	\$aaaAb	\$	Reduce $A \rightarrow aA$
8.	\$aa A b	\$	Reduce $A \rightarrow aA$
9.	\$a A b	\$	Reduce $A \rightarrow aA$
10.	\$A b	\$	Reduce $B \rightarrow \varepsilon$
11.	\$A b B	\$	Reduce $B \rightarrow bB$
12.	\$A B	\$	Reduce $S \rightarrow AB$
13.	\$S	\$	Accept

